## type_formation

        Γ⊢τ₁:⚹   Γ⊢τ₂:⚹        Γ,(α:κ)⊢τ:⚹
      -------------------    ---------------
           Γ⊢τ₁→τ₂:⚹            Γ⊢∀α:κ.τ:⚹


     Γ,(α:κ₁)⊢τ:κ₂         Γ⊢τ₁:κ₂→κ   Γ⊢τ₂:κ₂
  -------------------    -----------------------
    Γ⊢λα:κ₁.τ:κ₁→κ₂              Γ⊢τ₁τ₂:κ

## type_equivalence

                     τ ≡ σ        τ₁ ≡ τ₂   τ₂ ≡ τ₃
      ---------    ---------    ---------------------
        τ ≡ τ        σ ≡ τ             τ₁ ≡ τ₃


          τ₁ ≡ σ₁   τ₂ ≡ σ₂             τ ≡ σ
        ---------------------    -------------------
            τ₁→τ₂ ≡ σ₁→σ₂          ∀α:κ.τ ≡ ∀α:κ.σ


               τ ≡ σ             τ₁ ≡ σ₁   τ₂ ≡ σ₂
        -------------------    ---------------------
          λα:κ.τ ≡ λα:κ.σ           τ₁τ₂ ≡ σ₁σ₂



     -------------------------    ---------------------
       λα:κ.τ ≡ λβ:κ.τ[α:=β]        λα:κ.τσ ≡ τ[α:=σ]

## expression_formation

           x:τ ∈ Γ        Γ⊢τ₁:⚹   Γ,(x:τ₁)⊢e:τ₂
         -----------    --------------------------
            Γ⊢x:τ            Γ⊢λx:τ₁.e:τ₁→τ₂


         Γ⊢e₁:τ₂→τ   Γ⊢e₂:τ₂          Γ,(α:κ)⊢e:τ
       -----------------------    -------------------
               Γ⊢e₁e₂:τ             Γ⊢Λα:κ.e:∀α:κ.τ


      Γ⊢e:∀α:κ.τ   Γ⊢σ:κ        Γ⊢e:τ   τ ≡ σ   Γ⊢σ:⚹
    ----------------------    -------------------------
         Γ⊢eσ:τ[α:=σ]                   Γ⊢e:σ

## reduction

    λx:τ.ee₁ →→ e[x:=e₁]    Λα:κ.eτ →→ e[α:=τ]


           e₁ →→ e₂            e₁ →→ e₂
       ----------------    ----------------
         e₁e₃ →→ e₂e₃        e₃e₁ →→ e₃e₂


        e₁ →→ e₂              e₁ →→ e₂
     --------------    ----------------------
       e₁τ →→ e₂τ        λx:τ.e₁ →→ λx:τ.e₂


                     e₁ →→ e₂
              ----------------------
                Λα:κ.e₁ →→ Λα:κ.e₂

